---
title: 'DSP notes'
date: 2023-10-01
permalink: /posts/2023/10/DSP-notes/
tags:
  - UF
---


$$\section{DTFT Time Reversal Property: Variable Substitution Method}$$

$$\subsection{Core Concept: Variable Substitution}$$

When we substitute variables in an equation, we're essentially relabeling our terms without changing the mathematical result. Think of it like renaming items in a list---the content stays the same, just the labels change.

$$\subsection{DTFT Time Reversal Proof (Step-by-Step)}$$

$$\textbf{Starting Point:}$$
We want to find the DTFT of a time-reversed signal $$x[-n]$$:

$$\begin{equation}
\text{DTFT}(x[-n]) = \sum_{n=-\infty}^{\infty} x[-n]e^{-j\omega n}
\end{equation}$$

$$\textbf{Step 1: Variable Substitution}$$
Let $$k = -n$$, which means $$n = -k$$

$$\textbf{Step 2: Rewrite the Sum}$
When $$n = -k$$, our sum becomes:
$$\begin{equation}
\sum_{k=-\infty}^{\infty} x[k]e^{-j\omega(-k)} = \sum_{k=-\infty}^{\infty} x[k]e^{j\omega k}
\end{equation}$$


------